{
  "@context": {
    "rdf": "http://www.w3.org/1999/02/22-rdf-syntax-ns#",
    "rdfs": "http://www.w3.org/2000/01/rdf-schema#",
    "schema": "http://schema.org/",
    "webiot": "http://schema.webizing.org/",
    "xsd": "http://www.w3.org/2001/XMLSchema#"
  },
  "@graph": [
    {
      "@id": "webiot:startDate",
      "@type": "rdf:Property",
      "rdfs:comment": "\n                        start time ex)2017-09-10T00:00:00+09:00\n                    ",
      "rdfs:label": "\n                            startDate\n                        ",
      "schema:rangeIncludes": {
        "@id": "schema:DateTime"
      }
    },
    {
      "@id": "webiot:standHour",
      "@type": "rdf:Property",
      "rdfs:comment": "\n                        일어선 시간 - 1: 1시간, 0: 0시간\n                    ",
      "rdfs:label": "\n                            standHour\n                        ",
      "schema:rangeIncludes": {
        "@id": "schema:Float"
      }
    },
    {
      "@id": "webiot:stepCount",
      "@type": "rdf:Property",
      "rdfs:comment": "\n                        걸음 수\n                    ",
      "rdfs:label": "\n                            stepCount\n                        ",
      "schema:rangeIncludes": {
        "@id": "schema:Integer"
      }
    },
    {
      "@id": "webiot:heartRate",
      "@type": "rdf:Property",
      "rdfs:comment": "\n                        심박수 - unit: count/min\n                    ",
      "rdfs:label": "\n                            heartRate\n                        ",
      "schema:rangeIncludes": {
        "@id": "schema:Integer"
      }
    },
    {
      "@id": "webiot:SmartWatch",
      "@type": "rdfs:Class",
      "rdfs:comment": "\n            SmartWatch Sensor - 걸음 수, 심박, 운동시간, 일어서 있는 시간 로깅 ex)Fitbit, AppleWatch\n        ",
      "rdfs:label": "SmartWatch",
      "schema:sameAs": {
        "@id": "webiot:SmartWatch"
      }
    },
    {
      "@id": "webiot:address",
      "@type": "rdf:Property",
      "rdfs:comment": "\n                        building where the sensor resides - format: organization-building ex)yongjaelee-house, kist-l1, kist-l8\n                    ",
      "rdfs:label": "\n                            address\n                        ",
      "schema:rangeIncludes": {
        "@id": "schema:Text"
      }
    },
    {
      "@id": "webiot:location",
      "@type": "rdf:Property",
      "rdfs:comment": "\n                        location of the sensor - format: free\n                    ",
      "rdfs:label": "\n                            location\n                        ",
      "schema:rangeIncludes": {
        "@id": "schema:Text"
      }
    },
    {
      "@id": "webiot:user",
      "@type": "rdf:Property",
      "rdfs:comment": "\n                        user of the sensor - format: firstName+LastName ex)jonghoLee, wanhoIm\n                    ",
      "rdfs:label": "\n                            user\n                        ",
      "schema:rangeIncludes": {
        "@id": "schema:Text"
      }
    },
    {
      "@id": "webiot:exerciseTime",
      "@type": "rdf:Property",
      "rdfs:comment": "\n                        운동시간 - unit: minute\n                    ",
      "rdfs:label": "\n                            exerciseTime\n                        ",
      "schema:rangeIncludes": {
        "@id": "schema:Float"
      }
    },
    {
      "@id": "webiot:endDate",
      "@type": "rdf:Property",
      "rdfs:comment": "\n                        sleep end time ex)2017-09-10T06:30:00+09:00\n                    ",
      "rdfs:label": "\n                            endDate\n                        ",
      "schema:rangeIncludes": {
        "@id": "schema:DateTime"
      }
    },
    {
      "@id": "webiot:time",
      "@type": "rdf:Property",
      "rdfs:comment": "\n                        time at which the data measurement was made - ex)\"2017-05-30T18:54:20+09:00\"\n                    ",
      "rdfs:label": "\n                            time\n                        ",
      "schema:rangeIncludes": {
        "@id": "schema:DateTime"
      }
    },
    {
      "@id": "webiot:name",
      "@type": "rdf:Property",
      "rdfs:comment": "\n                        name of the sensor - format: SensorXX ex)Foobot00, Beddit02\n                    ",
      "rdfs:label": "\n                            name\n                        ",
      "schema:rangeIncludes": {
        "@id": "schema:Text"
      }
    },
    {
      "@id": "webiot:room",
      "@type": "rdf:Property",
      "rdfs:comment": "\n                        room number of the building where the sensor resides - ex) L8321\n                    ",
      "rdfs:label": "\n                            room\n                        ",
      "schema:rangeIncludes": {
        "@id": "schema:Text"
      }
    }
  ]
}