{
  "@context": {
    "rdf": "http://www.w3.org/1999/02/22-rdf-syntax-ns#",
    "rdfs": "http://www.w3.org/2000/01/rdf-schema#",
    "schema": "http://schema.org/",
    "webiot": "http://schema.webizing.org/",
    "xsd": "http://www.w3.org/2001/XMLSchema#"
  },
  "@graph": [
    {
      "@id": "webiot:SmartTable",
      "@type": "rdfs:Class",
      "rdfs:comment": "\n            SmartTable Sensor - 음식 리스트, 음식 칼로리, 사진 URL 로깅\n        ",
      "rdfs:label": "SmartTable",
      "schema:sameAs": {
        "@id": "webiot:SmartTable"
      }
    },
    {
      "@id": "webiot:caloryList",
      "@type": "rdf:Property",
      "rdfs:comment": "\n                        List of calories for the food items\n                    ",
      "rdfs:label": "\n                            caloryList\n                        ",
      "schema:rangeIncludes": {
        "@id": "schema:ItemList"
      }
    },
    {
      "@id": "webiot:location",
      "@type": "rdf:Property",
      "rdfs:comment": "\n                        location of the sensor - format: free\n                    ",
      "rdfs:label": "\n                            location\n                        ",
      "schema:rangeIncludes": {
        "@id": "schema:Text"
      }
    },
    {
      "@id": "webiot:foodList",
      "@type": "rdf:Property",
      "rdfs:comment": "\n                        List of food items\n                    ",
      "rdfs:label": "\n                            foodList\n                        ",
      "schema:rangeIncludes": {
        "@id": "schema:ItemList"
      }
    },
    {
      "@id": "webiot:address",
      "@type": "rdf:Property",
      "rdfs:comment": "\n                        building where the sensor resides - format: organization-building ex)yongjaelee-house, kist-l1, kist-l8\n                    ",
      "rdfs:label": "\n                            address\n                        ",
      "schema:rangeIncludes": {
        "@id": "schema:Text"
      }
    },
    {
      "@id": "webiot:room",
      "@type": "rdf:Property",
      "rdfs:comment": "\n                        room number of the building where the sensor resides - ex) L8321\n                    ",
      "rdfs:label": "\n                            room\n                        ",
      "schema:rangeIncludes": {
        "@id": "schema:Text"
      }
    },
    {
      "@id": "webiot:user",
      "@type": "rdf:Property",
      "rdfs:comment": "\n                        user of the sensor - format: firstName+LastName ex)jonghoLee, wanhoIm\n                    ",
      "rdfs:label": "\n                            user\n                        ",
      "schema:rangeIncludes": {
        "@id": "schema:Text"
      }
    },
    {
      "@id": "webiot:time",
      "@type": "rdf:Property",
      "rdfs:comment": "\n                        time at which the data measurement was made - ex)\"2017-05-30T18:54:20+09:00\"\n                    ",
      "rdfs:label": "\n                            time\n                        ",
      "schema:rangeIncludes": {
        "@id": "schema:DateTime"
      }
    },
    {
      "@id": "webiot:name",
      "@type": "rdf:Property",
      "rdfs:comment": "\n                        name of the sensor - format: SensorXX ex)Foobot00, Beddit02\n                    ",
      "rdfs:label": "\n                            name\n                        ",
      "schema:rangeIncludes": {
        "@id": "schema:Text"
      }
    },
    {
      "@id": "webiot:snapShot",
      "@type": "rdf:Property",
      "rdfs:comment": "\n                        url of the snap shot of the table\n                    ",
      "rdfs:label": "\n                            snapShot\n                        ",
      "schema:rangeIncludes": {
        "@id": "schema:URL"
      }
    }
  ]
}